\subsubsection*{Stationary-State Case}
    Consider first the stationary state system. \cite{LHF22} considers the incompressible limit, where $\rho_{M}$ is constant, $\rmEu  =  2$, and the energy conservation equation (\ref{eqn:energy conservation}) is discounted. The authors consider test functions for each equation in the space:\footnote{The notation there differs slightly.}
    \begin{center}\begin{tabular}{ r l c | c }
        \multicolumn{2}{c}{Equation}  &  Index  &  Test space  \\
        \hline\hline
        Mass conservation  &  $0  =  \nabla\cdot\bfp$  &  (\ref{eqn:mass conservation})  &  $\calP$  \\
        Momentum conservation  &  $\bfzero 
         =  - \nabla\cdot\left[\bfp^{\otimes 2}\right] - \nabla p + \frac{2}{\beta}\bfj\wedge\bfB + \frac{1}{\rmRef}\Delta\bfp$  &  (\ref{eqn:momentum conservation})  &  $\calU$  \\
        \hline
        Current identity  &  $\bfzero  =  \frac{1}{\rmRem}\bfj - (\bfE + \bfp\wedge\bfB) + \rmRH\bfj\wedge\bfB$  &  (\ref{eqn:current identity})  &  $\calJ$  \\
        \hline
        Ampère's law  &  $\bfzero  =  \nabla\wedge\bfB - \bfj$  &  (\ref{eqn:Ampère's law})  &  $\calE$  \\
        Faraday's law  &  $\bfzero  =  \nabla\wedge\bfE$  &  (\ref{eqn:Faraday's law})  &  $\calB$  \\
        Gauss's law  &  $\bfzero  =  \nabla\cdot\bfB$  &  (\ref{eqn:Gauss's law})  &  $\nabla\cdot\calB$  \\
    \end{tabular}\end{center}
    We than have the variational formulation: \BA{(Clear up and clarify the notation a little here, even if this way is informative and convenient.)}
    \begin{align}
        \forall q \in \calP,  0  &=  \langle\nabla\cdot\bfp, q\rangle_{\bfOmega}  \\
        \begin{split}
            \forall \bfq \in \calU,  0  &=  \left(\left\langle\bfp^{\otimes 2}, \nabla\bfq\right\rangle + \langle p, \nabla\cdot\bfq\rangle + \frac{2}{\beta}\langle\bfj\wedge\bfB, \bfq\rangle - \frac{1}{\rmRef}\langle\nabla\bfp, \nabla\bfq\rangle\right)_{\bfOmega}  \\
            &\;\;\;\;\;\;\;\;\;\;\;\;\;\;\;\;\;\;\;\;\;\;\;\;\;\;\;\;\;\;\;\;  + \left(- \langle(\bfp\cdot\bfn)\bfp, \bfq\rangle - \langle p, \bfq\cdot\bfn\rangle + \frac{1}{\rmRef}\langle\bfn\cdot\nabla\bfp, \nabla\bfq\rangle\right)_{\bfGamma}
        \end{split}  \\
        \forall \bfk \in \calJ,  0  &=  \left(\frac{1}{\rmRem}\langle\bfj, \bfk\rangle - \langle\bfE, \bfk\rangle - \langle\bfp\wedge\bfB, \bfk\rangle + \rmRH\langle\bfj\wedge\bfB, \bfk\rangle\right)_{\bfOmega}  \\
        \forall \bfF \in \calE,  0  &=  \left(\langle\bfB, \nabla\wedge\bfF\rangle - \langle\bfj, \bfF\rangle\tall\right)_{\bfOmega} - \langle\bfB\wedge\bfn, \bfF\rangle_{\bfGamma}  \\
        \forall \bfC \in \calB,  0  &=  \left(\langle\nabla\wedge\bfE, \bfC\rangle + \langle\nabla\cdot\bfB, \nabla\cdot\bfC\rangle\tall\right)_{\bfOmega}
    \end{align}
    